Test both incremental an standalone modes with the same input

code/experimental/sha256/Hacl.Test.Hash.SHA2.fst
@@ -5,10 +5,10 @@ open FStar.Buffer
 module SHA2 = Hacl.Hash.SHA2.L256
 
 
-val main: unit -> ST FStar.Int32.t
+val test_1: unit -> ST unit
   (requires (fun h -> True))
   (ensures  (fun h0 r h1 -> True))
-let main () =
+let test_1 () =
 
   (* Push a new memory frame *)
   (**) push_frame();
@@ -33,7 +33,45 @@ let main () =
   C.print_bytes output 32ul;
 
   (* Pop the memory frame *)
-  (**) pop_frame();
+  (**) pop_frame()
+
+
+val test_2: unit -> ST unit
+  (requires (fun h -> True))
+  (ensures  (fun h0 r h1 -> True))
+let test_2 () =
+
+  (* Push a new memory frame *)
+  (**) push_frame();
+
+  let output_len = 32ul in
+  let output = FStar.Buffer.create 0uy output_len in
+
+  let plaintext_len = 3ul in
+  let plaintext = FStar.Buffer.createL [
+      0x61uy; 0x62uy; 0x63uy;
+    ] in
+
+  (* Allocate memory for state *)
+  let ctx = FStar.Buffer.create 0ul 137ul in
+
+  (* Call the hash function *)
+  SHA2.sha256 output plaintext plaintext_len;
+
+  (* Display the result *)
+  C.print_bytes output 32ul;
+
+  (* Pop the memory frame *)
+  (**) pop_frame()
+
+
+
+val main: unit -> ST FStar.Int32.t
+  (requires (fun h -> True))
+  (ensures  (fun h0 r h1 -> True))
+let main () =
+  test_1 ();
+  test_2 ();
 
   (* Exit the program *)
   C.exit_success
